convert ttbenchmark to uint64, add notes to wishlist, update tttree to new Maps API, fix some bugs in SSTable

examples/ttbenchmark.dfy
@@ -1,31 +1,51 @@
+include "../lib/NativeTypes.dfy"
 include "tttree.dfy"
 
-module Integer_TTTree refines TwoThreeTree {
-    import Keyspace = Integer_Order
+import opened NT = NativeTypes
+
+module uint64_Order refines Total_Order {
+  import opened NativeTypes
+  type Element = uint64
+
+  predicate method lte(a: Element, b: Element) {
+    reveal_ltedef();
+    ltedef(a, b)
+  }
+
+  predicate method {:opaque} ltedef(a: Element, b: Element) {
+    a <= b
+  }
 }
 
-module Seq_Int_TTTree refines TwoThreeTree {
-    import Keyspace = Seq_Int_Lex_Order
+module uint64_TTTree refines TwoThreeTree {
+  import Keyspace = uint64_Order
 }
 
-module Seq_Char_TTTree refines TwoThreeTree {
-    import Keyspace = Seq_Char_Lex_Order
-}
+// module Integer_TTTree refines TwoThreeTree {
+//     import Keyspace = Integer_Order
+// }
 
-module String_TTTree refines TwoThreeTree {
-    import Keyspace = String_Lex_Order
-}
+// module Seq_Int_TTTree refines TwoThreeTree {
+//     import Keyspace = Seq_Int_Lex_Order
+// }
 
+// module Seq_Char_TTTree refines TwoThreeTree {
+//     import Keyspace = Seq_Char_Lex_Order
+// }
+
+// module String_TTTree refines TwoThreeTree {
+//     import Keyspace = String_Lex_Order
+// }
 
 method Main() {
-    var nInsertions := 1000 * 1000 * 10;
-    var t := Integer_TTTree.Tree.EmptyTree;
-    var i := 0;
+    var nInsertions: uint64 := 1000 * 1000 * 10;
+    var t := uint64_TTTree.Tree.EmptyTree;
+    var i: uint64 := 0;
     while i < nInsertions
-        invariant Integer_TTTree.TTTree(t);
+        invariant uint64_TTTree.TTTree(t);
     {
-        var v := (i * 1073741827) % nInsertions;
-        t := Integer_TTTree.Insert(t, v, v*v);
+        var v: uint64 := (i * 1073741827) % nInsertions;
+        t := uint64_TTTree.Insert(t, v, v);
         i := i + 1;
     }
 }
